theories/lifetime/model/definitions.v
@@ -4,9 +4,11 @@ From lrust.lifetime Require Export lifetime_sig.
 Set Default Proof Using "Type".
 Import uPred.
 
-Definition borN : namespace := lftN .@ "bor".
 Definition inhN : namespace := lftN .@ "inh".
 Definition mgmtN : namespace := lftN .@ "mgmt".
+(** We put borrows into the "user" namespace, so that they are available
+in [lft_vs]. *)
+Definition borN : namespace := lft_userN .@ "bor".
 
 Definition atomic_lft := positive.
 (* HACK : We need to make sure this is not in the top-level context,
@@ -140,7 +142,7 @@ Section defs.
        own_cnt κ (● n) ∗
        ∀ I : gmap lft lft_names,
          lft_vs_inv_go κ lft_inv_alive I -∗ ▷ Pb -∗ lft_dead κ
-           ={↑borN}=∗
+           ={↑lft_userN}=∗
          lft_vs_inv_go κ lft_inv_alive I ∗ ▷ Pi ∗ own_cnt κ (◯ n))%I.
 
   Definition lft_inv_alive_go (κ : lft)
@@ -268,7 +270,7 @@ Lemma lft_vs_unfold κ Pb Pi :
   lft_vs κ Pb Pi ⊣⊢ ∃ n : nat,
     own_cnt κ (● n) ∗
     ∀ I : gmap lft lft_names,
-      lft_vs_inv κ I -∗ ▷ Pb -∗ lft_dead κ ={↑borN}=∗
+      lft_vs_inv κ I -∗ ▷ Pb -∗ lft_dead κ ={↑lft_userN}=∗
       lft_vs_inv κ I ∗ ▷ Pi ∗ own_cnt κ (◯ n).
 Proof. done. Qed.
 
